NLustreToSyBloc/Translation.v
@@ -25,7 +25,7 @@ Module Type TRANSLATION
        (Import Clks    : CLOCKS   Ids)
        (Import ExprSyn : NLEXPRSYNTAX Op)
        (Import SynNL   : NLSYNTAX Ids Op Clks ExprSyn)
-       (SynSB          : SBSYNTAX Ids Op)
+       (SynSB          : SBSYNTAX Ids Op Clks ExprSyn)
        (Import Mem     : MEMORIES Ids Op Clks ExprSyn SynNL).
 
   Definition gather_eq (acc: list (ident * const) * list (ident * ident)) (eq: equation):
@@ -75,66 +75,64 @@ Module Type TRANSLATION
 
   Section Translate.
 
-    Variable memories : Environment.t const.
+    (* Variable memories : Environment.t const. *)
 
-    Definition tovar (x: ident) : SynSB.var :=
-      if Environment.mem x memories then SynSB.Last x else SynSB.Var x.
+    (* Definition tovar (x: ident) : SynSB.var := *)
+    (*   if Environment.mem x memories then SynSB.Last x else SynSB.Var x. *)
 
-    Fixpoint translate_lexp (e: lexp) : SynSB.lexp :=
-      match e with
-      | Econst c          => SynSB.Econst c
-      | Evar x ty         => SynSB.Evar (tovar x) ty
-      | Ewhen e x k       => SynSB.Ewhen (translate_lexp e) (tovar x) k
-      | Eunop o e ty      => SynSB.Eunop o (translate_lexp e) ty
-      | Ebinop o e1 e2 ty => SynSB.Ebinop o (translate_lexp e1) (translate_lexp e2) ty
-      end.
-
-    Fixpoint translate_cexp (e: cexp) : SynSB.cexp :=
-      match e with
-      | Emerge x e1 e2 => SynSB.Emerge (tovar x) (translate_cexp e1) (translate_cexp e2)
-      | Eite e e1 e2   => SynSB.Eite (translate_lexp e) (translate_cexp e1) (translate_cexp e2)
-      | Eexp e         => SynSB.Eexp (translate_lexp e)
-      end.
-
-    (* Definition init (ck: clock) : ident. *)
-    (* Admitted. *)
-
-    (* Definition state (x: ident) : ident. *)
-    (* Admitted. *)
-
-    (* Definition op_or : binop. *)
-    (* Admitted. *)
-
-    (* Definition reset_expr (r: option (ident * clock)) (init: ident) : SynSB.lexp := *)
-    (*   match r with *)
-    (*   | Some (r, ck_r) => *)
-    (*     SynSB.Ebinop op_or (SynSB.Evar (SynSB.Last init) bool_type) (SynSB.Evar (tovar r) bool_type) bool_type *)
-    (*   | None => *)
-    (*     SynSB.Evar (SynSB.Last init) bool_type *)
+    (* Fixpoint translate_lexp (e: lexp) : SynSB.lexp := *)
+    (*   match e with *)
+    (*   | Econst c          => SynSB.Econst c *)
+    (*   | Evar x ty         => SynSB.Evar (tovar x) ty *)
+    (*   | Ewhen e x k       => SynSB.Ewhen (translate_lexp e) (tovar x) k *)
+    (*   | Eunop o e ty      => SynSB.Eunop o (translate_lexp e) ty *)
+    (*   | Ebinop o e1 e2 ty => SynSB.Ebinop o (translate_lexp e1) (translate_lexp e2) ty *)
     (*   end. *)
 
-    Fixpoint translate_clock (ck: clock) : SynSB.clock :=
-      match ck with
-      | Cbase => SynSB.Cbase
-      | Con ck x k => SynSB.Con (translate_clock ck) (tovar x) k
-      end.
+    (* Fixpoint translate_cexp (e: cexp) : SynSB.cexp := *)
+    (*   match e with *)
+    (*   | Emerge x e1 e2 => SynSB.Emerge (tovar x) (translate_cexp e1) (translate_cexp e2) *)
+    (*   | Eite e e1 e2   => SynSB.Eite (translate_lexp e) (translate_cexp e1) (translate_cexp e2) *)
+    (*   | Eexp e         => SynSB.Eexp (translate_lexp e) *)
+    (*   end. *)
+
+    (* (* Definition init (ck: clock) : ident. *) *)
+    (* (* Admitted. *) *)
+
+    (* (* Definition state (x: ident) : ident. *) *)
+    (* (* Admitted. *) *)
+
+    (* (* Definition op_or : binop. *) *)
+    (* (* Admitted. *) *)
+
+    (* (* Definition reset_expr (r: option (ident * clock)) (init: ident) : SynSB.lexp := *) *)
+    (* (*   match r with *) *)
+    (* (*   | Some (r, ck_r) => *) *)
+    (* (*     SynSB.Ebinop op_or (SynSB.Evar (SynSB.Last init) bool_type) (SynSB.Evar (tovar r) bool_type) bool_type *) *)
+    (* (*   | None => *) *)
+    (* (*     SynSB.Evar (SynSB.Last init) bool_type *) *)
+    (* (*   end. *) *)
+
+    (* Fixpoint translate_clock (ck: clock) : SynSB.clock := *)
+    (*   match ck with *)
+    (*   | Cbase => SynSB.Cbase *)
+    (*   | Con ck x k => SynSB.Con (translate_clock ck) (tovar x) k *)
+    (*   end. *)
 
     Definition translate_eqn (eqn: equation) : list SynSB.equation :=
       match eqn with
       | EqDef x ck e =>
-        [ SynSB.EqDef x (translate_clock ck) (translate_cexp e) ]
+        [ SynSB.EqDef x ck e ]
       | EqApp xs ck f les None =>
         let s := hd Ids.default xs in
-        let ck := translate_clock ck in
         [ SynSB.EqTransient s ck;
-          SynSB.EqCall s xs ck f (map translate_lexp les) ]
+          SynSB.EqCall s xs ck f les ]
       | EqApp xs ck f les (Some (r, ck_r)) =>
         let s := hd Ids.default xs in
-        let ck := translate_clock ck in
-        [ SynSB.EqReset s ck f (tovar r);
-          SynSB.EqCall s xs ck f (map translate_lexp les) ]
+        [ SynSB.EqReset s ck f r;
+          SynSB.EqCall s xs ck f les ]
       | EqFby x ck _ e =>
-        [ SynSB.EqNext x (translate_clock ck) (translate_lexp e) ]
+        [ SynSB.EqNext x ck e ]
       end.
 
   (*   (** Remark: eqns ordered in reverse order of execution for coherence with *)
@@ -649,7 +647,7 @@ Module Type TRANSLATION
        SynSB.b_vars := idty vars;
        SynSB.b_lasts := lasts;
        SynSB.b_out  := idty n.(n_out);
-       SynSB.b_eqs  := translate_eqns lasts n.(n_eqs)
+       SynSB.b_eqs  := translate_eqns n.(n_eqs)
     |}.
   Next Obligation.
     destruct n; simpl.
@@ -717,7 +715,7 @@ Module TranslationFun
        (Clks    : CLOCKS Ids)
        (ExprSyn : NLEXPRSYNTAX Op)
        (SynNL   : NLSYNTAX Ids Op Clks ExprSyn)
-       (SynSB   : SBSYNTAX Ids Op)
+       (SynSB   : SBSYNTAX Ids Op Clks ExprSyn)
        (Mem     : MEMORIES Ids Op Clks ExprSyn SynNL)
 <: TRANSLATION Ids Op Clks ExprSyn SynNL SynSB Mem.
   Include TRANSLATION Ids Op Clks ExprSyn SynNL SynSB Mem.
