SyBloc/SBSyntax.v
@@ -1,5 +1,7 @@
 Require Import Velus.Common.
 Require Import Velus.Operators.
+Require Import Velus.NLustre.NLExprSyntax.
+Require Import Velus.Clocks.
 
 Require Import List.
 Import List.ListNotations.
@@ -7,56 +9,16 @@ Open Scope list_scope.
 
 Module Type SBSYNTAX
        (Import Ids     : IDS)
-       (Import Op      : OPERATORS).
-
-  (** ** Expressions *)
-
-  Inductive var : Type :=
-  | Var  : ident -> var
-  | Last : ident -> var.
-
-  Inductive lexp : Type :=
-  | Econst : const -> lexp
-  | Evar   : var -> type -> lexp
-  | Ewhen  : lexp -> var -> bool -> lexp
-  | Eunop  : unop -> lexp -> type -> lexp
-  | Ebinop : binop -> lexp -> lexp -> type -> lexp.
-
-  Definition lexps := list lexp.
-
-  (** ** Control expressions *)
-
-  Inductive cexp : Type :=
-  | Emerge : var -> cexp -> cexp -> cexp
-  | Eite   : lexp -> cexp -> cexp -> cexp
-  | Eexp   : lexp -> cexp.
-
-  (** ** State expressions *)
-
-  (* Inductive sexp : Type := *)
-  (* | ESlast  : ident -> sexp *)
-  (* | ESite   : lexp -> sexp -> sexp -> sexp *)
-  (* | ESreset : ident -> sexp. *)
-
-  Fixpoint typeof (le: lexp): type :=
-    match le with
-    | Econst c => type_const c
-    | Evar _ ty
-    | Eunop _ _ ty
-    | Ebinop _ _ _ ty => ty
-    | Ewhen e _ _ => typeof e
-    end.
-
-  Inductive clock : Type :=
-  | Cbase : clock
-  | Con   : clock -> var -> bool -> clock.
+       (Import Op      : OPERATORS)
+       (Import Clks    : CLOCKS       Ids)
+       (Import ExprSyn : NLEXPRSYNTAX     Op).
 
   (** ** Equations *)
 
   Inductive equation :=
   | EqDef       : ident -> clock -> cexp -> equation
   | EqNext      : ident -> clock -> lexp -> equation
-  | EqReset     : ident -> clock -> ident -> var -> equation
+  | EqReset     : ident -> clock -> ident -> ident -> equation
   (* <trans s> =ck reset block<last s> on e *)
   | EqTransient : ident -> clock -> equation
   | EqCall      : ident -> idents -> clock -> ident -> list lexp -> equation.
@@ -191,6 +153,8 @@ End SBSYNTAX.
 Module SBSyntaxFun
        (Ids  : IDS)
        (Op   : OPERATORS)
-       <: SBSYNTAX Ids Op.
-  Include SBSYNTAX Ids Op.
+       (Clks : CLOCKS          Ids)
+       (ExprSyn : NLEXPRSYNTAX     Op)
+       <: SBSYNTAX Ids Op Clks ExprSyn.
+  Include SBSYNTAX Ids Op Clks ExprSyn.
 End SBSyntaxFun.
